---
tags:
  - set
  - theory
mathLink: intersection under preimage proposition
---
> [!prop]
> The [[Intersection]] behaves nicely under the [[Preimage]]:
> $f^{-1}\left(\bigcap_{\lambda\in\Lambda}U_\lambda\right)=\bigcap_{\lambda\in\Lambda}f^{-1}(U_\lambda)$

> [!proof]
> Let $x\in f^{-1}(\bigcup_{\lambda\in\Lambda}U_\lambda)$ be given.
> Then, pick $\lambda\in\Lambda$ with $f(x)\in U_\lambda$. $x\in f^{-1}(U_\lambda)$, so $x\in \bigcup_{\lambda\in\Lambda}f^{-1}(U_\lambda)$. 
> [[therefore]] $f^{-1}(\bigcup_{\lambda\in\Lambda}U_\lambda)$ [[subset]] $\bigcup_{\lambda\in\Lambda}f^{-1}(U_\lambda)$
> Let $x\in\bigcup_{\lambda\in\Lambda}f^{-1}(U_\lambda)$ be given.
> Then, pick $\lambda\in\Lambda$ with $x\in f^{-1}(U_\lambda)$ . $f(x)\in\bigcup_{\lambda\in\Lambda}U_\lambda$, so $x\in f^{-1}\left(\bigcup_{\lambda\in\Lambda}U_\lambda\right)$.
> [[therefore]] $\bigcup_{\lambda\in\Lambda}f^{-1}(U_\lambda)$ [[subset]] $f^{-1}\left(\bigcup_{\lambda\in\Lambda}U_\lambda\right)$.
