---
tag: set theory
mathLink: union under inverse image lemma
---
```ad-prop
The [[Set Theory/Union|Union]] behaves nicely under the [[Set Theory/Preimage|Preimage]]:
$$f^{-1}\left(\bigcup_{\lambda\in\Lambda}U_\lambda\right)=\bigcup_{\lambda\in\Lambda}f^{-1}(U_\lambda)$$
```

```ad-proof
Let $x\in f^{-1}(\bigcap_{\lambda\in\Lambda}U_\lambda)$ be given.
Then, $\forall\lambda\in\Lambda: f(x)\in U_\lambda$. So, $\forall\lambda:x\in f^{-1}(U_\lambda)$, so $x\in \bigcap_{\lambda\in\Lambda}f^{-1}(U_\lambda)$. 
[[therefore]] $f^{-1}(\bigcap_{\lambda\in\Lambda}U_\lambda)$ [[Notation/subset|subset]] $\bigcap_{\lambda\in\Lambda}f^{-1}(U_\lambda)$
Let $x\in\bigcap_{\lambda\in\Lambda}f^{-1}(U_\lambda)$ be given.
Then, $\forall\lambda\in\Lambda:x\in f^{-1}(U_\lambda)$ . $\forall\lambda:f(x)\in\bigcup_{\lambda\in\Lambda}U_\lambda$, so $x\in f^{-1}\left(\bigcap_{\lambda\in\Lambda}U_\lambda\right)$.
[[therefore]] $\bigcap_{\lambda\in\Lambda}f^{-1}(U_\lambda)$ [[Notation/subset|subset]] $f^{-1}\left(\bigcap_{\lambda\in\Lambda}U_\lambda\right)$.
```

