# Dumbbell Model
- two beads connected by a spring
- center of mass: $r_{c}= \frac{1}{2}(r_{1}+r_{2})$
- end-to-end: $q=r_{2}-r_{1}$

Homogeneous flows:
- rate of strain tensor is independent of position

$$\dot \gamma=\nabla v+(\nabla v)^{T}$$
velocity: $$v(r)=v_{0}+(\nabla v)^{T}\cdot r$$
$$\kappa=(\nabla v)^{T}$$
incompressability: 
$$\kappa_{xx}+\kappa_{yy}+\kappa_{zz}=0$$
Simple shear flow:
- shear rate $$\dot \gamma$$
- $v_{x}=\kappa_{xy}y$
- $v_{y}=0$
- $v_{z}=0$

Shear free flow:
- $v_{x}= - \frac{1}{2}\kappa_{zz}(1+b)$
- $v_{y}=- \frac{1}{2}\kappa_{zz}(1-b)$
- $v_{z}=\kappa_{zz}z$
- with parameter $0≤b≤1$
- elongation rate $\dot \epsilon$

# Non-Equilibrium Distribution of the Dumbbell
Distribution: $$F(\dot r_{1},\dot r_{2},Q,t)$$
Configuration distribution function: $$\Psi^{-}(Q,t)=\int F(\dot r,Q,t)\ d\dot r$$
Momentum space distribution function: $$\Xi(\dot r,Q,t)=\frac{F(\dot r,Q,t)}{\Psi(Q,t)}$$
Assume $\Xi$ is Maxwellian WRT solvent velocity field: 
$$\Xi= \frac{e^{- \frac{1}{2}\sum_{\nu=1}^{2}m[(\dot r_{1}-v)^{2}+(\dot r_{2}-v)^{2}]}}{Z}$$where $Z$ is the normalizing [[Partition Function]]. This assumption is called equilibration in momentum space.

We can write: $$F(\dot r_{1},\dot r_{2},Q,t)=\Xi(\dot r_{1},\dot r_{2},Q,t)\Psi(Q,t)$$
For an operator $B$, the expected value is $\langle B\rangle$ and the momentum space expected value is $\langle B\rangle_{p}$

Stress Tensor:
- Stress is force per unit area
- $\sigma_{T}=n\cdot \Pi$. where $\sigma_{T}$ is the stress force, $n$ is a unit normal vector to the surface, and $\Pi$ is the stress tensor matrix

Assume $\Pi=\Pi_{S}+\Pi_{P}$, a contribution of the solvent and the polymer
$$\Pi_{S}=P_{S}\delta-\eta_{S}\dot \gamma$$where $\delta$ is the identity matrix (given by [[Kronecker-Delta]]).

$$\Pi_{P}=P_{p}\delta+\tau_{p}$$




Hydrodynamic drag force: $$F_{i}^{(h)}=-\zeta(\langle\dot r_{i}\rangle_{p}-(v_{i}+v'_{i}))$$
$v_{i}'$ is the hydrodynamic interaction term

Brownian term: 
$$F_{i}^{(b)}= -k_{b}T \frac{\partial \ln \Psi}{\partial r_{i}}$$
Spring force: $$F_{i}^{(\phi)}=- \frac{\partial \phi}{\partial r_{i}}$$
External force: $F_{i}^{(e)}$

Balanced forces: $$0=F^{(h)}+F^{(b)}+F^{(\phi)}+F^{(e)}$$
we can rearrange to find $\dot r_{i}$:  $$\langle\dot r_{i}\rangle_{p}=v_{0}+ \kappa\cdot r_{i}- \frac{kT}{\zeta} \frac{\partial \ln \Psi}{\partial r_{i}}- \frac{1}{\zeta}\frac{\partial \phi}{\partial r_{i}}+ \frac{1}{\zeta}F_{i}^{(e)}$$
$$\frac{\partial \ln \Psi}{\partial r_{1}}= -\frac{\partial \ln \Psi}{\partial Q}$$
$$\frac{\partial \ln \Psi}{\partial r_{2}}= \frac{\partial \ln \Psi}{\partial Q}$$
We can find: $$\langle\dot r_{c}\rangle_{p}=v_{0}+\kappa r_{c}+ \frac{1}{\zeta}(F_{1}^{(e)}+F^{(e)}_{2})$$
$$\langle \dot Q\rangle_{p}=\kappa Q- \frac{2kT}{\zeta}\frac{\partial \ln \Psi}{\partial Q}- \frac{2}{\zeta}F^{(c )}$$
where $$F^{(c)}= \frac{\partial \phi}{\partial Q}$$
