>[!def]
>The $1$-dimensional *wave equation*: $$\frac{\partial ^{2}y}{\partial t^{2}}=c^{2}\frac{\partial ^{2}y}{\partial x^{2}}$$subject to the boundary conditions: $$\forall t:y(0,t)=y(l,t)$$for a string fixed at endpoints $0,l$.

>[!def]
>The constant $c$ in the [[Wave Equation]] is the *speed of propagation* of the [[Wave]]

d'Alembert's Solution to the [[Wave Equation]]:

write using the [[d'Alembert Operator]]
$$\left[\frac{\partial ^{2}}{\partial t^{2}}-c^{2}\frac{\partial ^{2}}{\partial x^{2}}\right]y(x,t)=0$$
Because the [[Kernel]] of the [[d'Alembert Operator]] is the solution to this equation, the collection of [[Wave]]s forms a [[Vector Space]]

For real numbers $A,B$:
$$\begin{align}(A-B)(A+B)&=A(A+B)-B(A+B) \quad(\text{distribute})\\
&=A^{2}+AB-BA-B^{2}\quad(\text{distribute})\\
&=A^{2}+AB-AB-B^{2}\quad(\text{commute})\\
&=A^{2}+B^{2}\quad(\text{addition associativity})
\end{align}$$
If $A,B$ were [[Linear Transformation]]s, the distributive steps still hold by the definition of [[Linear]]ity. 

Letting $y\in \mathcal{C}^{2}$, the commute step holds.


change coordinates: $u=x+ct,v=x-ct$. Then, $$\begin{align}\frac{\partial y}{\partial x}&=\frac{\partial y}{\partial u}\frac{\partial u}{\partial x}+\frac{\partial y}{\partial v}\frac{\partial v}{\partial x}=\frac{\partial y}{\partial u}+\frac{\partial y}{\partial v}\\
\frac{\partial y}{\partial t}&=\frac{\partial y}{\partial u}c-\frac{\partial y}{\partial v}c\\
c\frac{\partial }{\partial x}&=c\frac{\partial }{\partial u}+c\frac{\partial} {\partial v}\\
\frac{\partial }{\partial t}&=c\frac{\partial }{\partial u}-c\frac{\partial }{\partial v}\end{align}$$
So, $$\square y=\left(-2c\frac{\partial }{\partial v}\right)\left(2c\frac{\partial }{\partial u}\right)y=0$$
so [[Wave Equation]] is equivalent to $$\frac{\partial^{2} y}{\partial u\partial v}=0$$
Solve: 
$$\begin{align*}\frac{\partial}{\partial u}\left(\frac{\partial y}{\partial v}\right)=0\\
\implies \frac{\partial y}{\partial v}&=\text{const}=h(v),\text{ a continuous function}\\
\implies y&=\int h(v)\ dv+f(u)=g(v)+f(u)\\
&=f(x+ct)+g(y-ct)
\end{align*}$$
Apply [[Boundary Condition]] with $\lambda=ct$
$$\begin{align}
0&=f(ct)+g(-ct)\\
&\quad f(\lambda)=-g(-\lambda)\\
0&=f(\lambda+l)+g(\lambda-l)\\
&\quad f(\lambda+l)=-g(\lambda-l)=f(l-\lambda)
\end{align}$$
for all $\lambda$. Can also write $f(\lambda'+2l)=f(\lambda')$ where $\lambda'=\lambda-l$


So, [[Periodic]]ity arrises from the [[Boundary Condition]]s

For example, $$f(\lambda)=C\sin\left(\frac{n\pi\lambda}{l}\right),n\in \mathbb{N}$$
are all of the possible solutions arising from sine functions. The [[Wavelength]]s are given by $$\lambda_{n}= \frac{l}{n\pi}\cdot2\pi= \frac{2l}{n}$$The [[Frequency]]ies are given by $$\nu_{n}= \frac{n}{2l}\cdot c$$
The [[Fundamental Frequency]] is $\nu_{1}$


Prove: $$\sin \alpha+\sin \beta=\sin\left(\frac{\alpha+\beta}{2}\right)\cdot\cos\left(\frac{\alpha-\beta}{2}\right)$$Complexify:
write: $$\begin{align}
\alpha&=\frac{\alpha+\beta}{2} + \frac{\alpha-\beta}{2}=\gamma+\delta\\
\beta&= \frac{\alpha+\beta}{2}- \frac{\alpha-\beta}{2}=\gamma-\delta
\end{align}$$Then,$$e^{i\alpha}+e^{i\beta}=e^{i (\gamma+\delta)}+e^{i(\gamma-\delta)}=e^{i\gamma}(e^{i \delta}+e^{-i \delta})=e^{i \gamma}(2\cos \delta)$$
So,
$$\Im \text{m}(e^{i\alpha}+e^{i\beta})=2\cos \delta\sin \gamma$$

>[!note]
>$$\frac{e^{ix}+e^{-ix}}{2}=\cos x$$
>$$\frac{e^{ix}-e^{-ix}}{2i}=\sin x$$

Orthonormality Relations:
Note that both $e^{2\pi int}$ and __ are $1$-[[Periodic]]. So, we want the length of the interval to be the period
$$I_{n,m}=\int_{0}^{1} e^{2\pi int}\cdot \overline{e^{2 \pi i m t}}\ dt=\int_{0}^{1}e^{2\pi i(n-m)t}dt$$
Case 1: $m=n$, $$\int_{0}^{1}1dt=1$$
Case 2: $mâ‰ n$, $$\int_{0}^{1}e^{2\pi i(n-m)t}dt=\left. \frac{1}{2\pi i(n-m)}e^{2\pi i(n-m)t}\right|_{0}^{1}=0$$by periodicity of the original integrand. So, we get $$I_{n,m}=\delta_{n,m}$$

