$$f=f(t)$$
continuum frequency variable: $\nu\in \mathbb{R}$ gives [[Fourier Transform]] in analogy to [[Fourier Coefficient]]:
$$\hat f:\mathbb{R}\rightarrow \mathbb{C},\quad\hat f(\nu)=\int_{-\infty}^{\infty}f(t)~e^{-2\pi i \nu t}\ dt$$
Analogue of the inversion property: when does 
$$f(t)=\int_{-\infty}^{\infty}\hat f(\nu)~e^{-2\pi \nu t}\ d \nu$$hold?

Need to make this statement rigorous: restrict to [[L1 Function]]s $f$. Then, for all $\nu\in \mathbb{R}$, $$\int_{-\infty}^{\infty}|f(t)~e^{-2\pi i \nu t}|\ dt=\int_{-\infty}^{\infty}|f(t)|\ dt<\infty$$
A-priori bound for [[Fourier Transform]]: $$\left|\widehat f(\nu)\right|\le\|\widehat f\|_{\infty}\le \|f\|_{\mathcal{L}^{1}},\quad\text{for all }\nu\in \mathbb{R}$$
- "The frequency domain is bounded by the time domain"


[[Fourier Transform]] of the [[Gaussian]]: 
$$g(t)=e^{-\pi t^{2}}$$
Fix $\nu\in \mathbb{R}$ arbitrary. Compute 
$$\begin{align*}
\widehat g(\nu)&= \int_{-\infty}^{\infty}e^{-\pi t^{2}}e^{-2\pi i \nu t}\ dt\\
&= \int_{-\infty}^{\infty}e^{-\pi (t^{2}+2 i \nu t)}\ dt\\
&= \int_{\infty}^{\infty}e^{-\pi((t+i \nu)^{2}+\nu^{2})}\ dt\\
&= e^{-\pi \nu^{2}}\underbrace{\int_{-\infty}^{\infty} e^{-\pi u^{2}}\ du}_{=1}\quad(\text{change variables }u=t+i \nu)\\
&= e^{-\pi \nu^{2}}\\
&= g(\nu)
\end{align*}$$

Note that we used a complex change of variables (justified by [[Residue Theorem]] in $\mathbb{C}$-analysis)

Where we completed the square:
$$t^{2}+2i \nu t= (t^{2}+2i \nu t+i^{2} \nu^{2})-i^{2}\nu^{2}=(t+i \nu)^{2}+\nu^{2}$$

We have shown [[Gaussian Invariance]]: $$\widehat g=g$$

We compute the gaussian integral:
$$\begin{align*}
I^{2}&= \left(\int_{-\infty}^{\infty}g(x)\ dx\right)^{2}\\
&= \int_{-\infty}^{\infty}g(x)\ dx\cdot\int_{-\infty}^{\infty}g(y)\ dy\\
&= \int_{-\infty}^{\infty}\int_{-\infty}^{\infty}g(x)g(y)\ dx\ dy\quad(\text{Fubini's Theorem})\\
&= \int_{-\infty}^{\infty}\int_{-\infty}^{\infty}e^{-\pi x^{2}}e^{-\pi y^{2}}\ dx\ dy\\
&= \int_{-\infty}^{\infty}\int_{-\infty}^{\infty}e^{-\pi(x^{2}+y^{2})}\ dx\ dy\\
&= \int_{0}^{2\pi }\int_{0}^{\infty}e^{-\pi r^{2}}r\ dr\ d \theta\\
&= \int_{0}^{2\pi}d \theta\int_{0}^{\infty}e^{-u}\cdot \frac{1}{2\pi}\ d r\quad(\text{change variables }u=\pi r^{2})\\
&= -e^{-u}\bigg|_{0}^{\infty} \\
&= 1
\end{align*}$$


[[Uncertainty Principle]] for the [[Gaussian]]:
$$\widehat{g_\epsilon}= \frac{1}{\epsilon}g_{\frac{1}{\epsilon}},\quad\epsilon>0$$
